Moved snapshot generation to code/
and started work on testing snapshot through Tezos API

code/snapshot/Tezos.fst
@@ -10,5 +10,5 @@ open Hacl.Impl.Curve25519.Fields
 open Hacl.Impl.Curve25519.Generic
 
 
-let curve25519_64_ecdh shared my_priv their_pub =
-  Hacl.Curve25519_64.ecdh shared my_priv their_pub
+let curve25519_51_ecdh shared my_priv their_pub =
+  Hacl.Curve25519_51.ecdh shared my_priv their_pub
